cedar-lean/Cedar/Thm/Validation/Typechecker/UnaryApp.lean
@@ -15,8 +15,6 @@
 -/
 
 import Cedar.Thm.Validation.Typechecker.Basic
-import Cedar.Thm.Validation.Typechecker.Types
-
 
 /-!
 This file proves that typechecking of `.unaryApp` expressions is sound.
@@ -53,12 +51,7 @@ theorem type_of_not_is_sound {x₁ : Expr} {c₁ c₂ : Capabilities} {env : Env
   (h₁ : CapabilitiesInvariant c₁ request entities)
   (h₂ : RequestAndEntitiesMatchEnvironment env request entities)
   (h₃ : typeOf (Expr.unaryApp .not x₁) c₁ env = Except.ok (ty, c₂))
-  (ih : ∀ {c₁ c₂ : Capabilities} {env : Environment} {ty : CedarType} {request : Request} {entities : Entities},
-      CapabilitiesInvariant c₁ request entities →
-      RequestAndEntitiesMatchEnvironment env request entities →
-      typeOf x₁ c₁ env = Except.ok (ty, c₂) →
-      GuardedCapabilitiesInvariant x₁ c₂ request entities ∧
-      ∃ v, EvaluatesTo x₁ request entities v ∧ InstanceOfType v ty) :
+  (ih : TypeOfIsSound x₁) :
   GuardedCapabilitiesInvariant (Expr.unaryApp .not x₁) c₂ request entities ∧
   ∃ v, EvaluatesTo (Expr.unaryApp .not x₁) request entities v ∧ InstanceOfType v ty
 := by
@@ -112,12 +105,7 @@ theorem type_of_neg_is_sound {x₁ : Expr} {c₁ c₂ : Capabilities} {env : Env
   (h₁ : CapabilitiesInvariant c₁ request entities)
   (h₂ : RequestAndEntitiesMatchEnvironment env request entities)
   (h₃ : typeOf (Expr.unaryApp .neg x₁) c₁ env = Except.ok (ty, c₂))
-  (ih : ∀ {c₁ c₂ : Capabilities} {env : Environment} {ty : CedarType} {request : Request} {entities : Entities},
-      CapabilitiesInvariant c₁ request entities →
-      RequestAndEntitiesMatchEnvironment env request entities →
-      typeOf x₁ c₁ env = Except.ok (ty, c₂) →
-      GuardedCapabilitiesInvariant x₁ c₂ request entities ∧
-      ∃ v, EvaluatesTo x₁ request entities v ∧ InstanceOfType v ty) :
+  (ih : TypeOfIsSound x₁) :
   GuardedCapabilitiesInvariant (Expr.unaryApp .neg x₁) c₂ request entities ∧
   ∃ v, EvaluatesTo (Expr.unaryApp .neg x₁) request entities v ∧ InstanceOfType v ty
 := by
@@ -164,12 +152,7 @@ theorem type_of_mulBy_is_sound {x₁ : Expr} {k : Int64} {c₁ c₂ : Capabiliti
   (h₁ : CapabilitiesInvariant c₁ request entities)
   (h₂ : RequestAndEntitiesMatchEnvironment env request entities)
   (h₃ : typeOf (Expr.unaryApp (.mulBy k) x₁) c₁ env = Except.ok (ty, c₂))
-  (ih : ∀ {c₁ c₂ : Capabilities} {env : Environment} {ty : CedarType} {request : Request} {entities : Entities},
-      CapabilitiesInvariant c₁ request entities →
-      RequestAndEntitiesMatchEnvironment env request entities →
-      typeOf x₁ c₁ env = Except.ok (ty, c₂) →
-      GuardedCapabilitiesInvariant x₁ c₂ request entities ∧
-      ∃ v, EvaluatesTo x₁ request entities v ∧ InstanceOfType v ty) :
+  (ih : TypeOfIsSound x₁) :
   GuardedCapabilitiesInvariant (Expr.unaryApp (.mulBy k) x₁) c₂ request entities ∧
   ∃ v, EvaluatesTo (Expr.unaryApp (.mulBy k) x₁) request entities v ∧ InstanceOfType v ty
 := by
@@ -216,12 +199,7 @@ theorem type_of_like_is_sound {x₁ : Expr} {p : Pattern} {c₁ c₂ : Capabilit
   (h₁ : CapabilitiesInvariant c₁ request entities)
   (h₂ : RequestAndEntitiesMatchEnvironment env request entities)
   (h₃ : typeOf (Expr.unaryApp (.like p) x₁) c₁ env = Except.ok (ty, c₂))
-  (ih : ∀ {c₁ c₂ : Capabilities} {env : Environment} {ty : CedarType} {request : Request} {entities : Entities},
-      CapabilitiesInvariant c₁ request entities →
-      RequestAndEntitiesMatchEnvironment env request entities →
-      typeOf x₁ c₁ env = Except.ok (ty, c₂) →
-      GuardedCapabilitiesInvariant x₁ c₂ request entities ∧
-      ∃ v, EvaluatesTo x₁ request entities v ∧ InstanceOfType v ty) :
+  (ih : TypeOfIsSound x₁) :
   GuardedCapabilitiesInvariant (Expr.unaryApp (.like p) x₁) c₂ request entities ∧
   ∃ v, EvaluatesTo (Expr.unaryApp (.like p) x₁) request entities v ∧ InstanceOfType v ty
 := by
@@ -270,12 +248,7 @@ theorem type_of_is_is_sound {x₁ : Expr} {ety : EntityType} {c₁ c₂ : Capabi
   (h₁ : CapabilitiesInvariant c₁ request entities)
   (h₂ : RequestAndEntitiesMatchEnvironment env request entities)
   (h₃ : typeOf (Expr.unaryApp (.is ety) x₁) c₁ env = Except.ok (ty, c₂))
-  (ih : ∀ {c₁ c₂ : Capabilities} {env : Environment} {ty : CedarType} {request : Request} {entities : Entities},
-      CapabilitiesInvariant c₁ request entities →
-      RequestAndEntitiesMatchEnvironment env request entities →
-      typeOf x₁ c₁ env = Except.ok (ty, c₂) →
-      GuardedCapabilitiesInvariant x₁ c₂ request entities ∧
-      ∃ v, EvaluatesTo x₁ request entities v ∧ InstanceOfType v ty) :
+  (ih : TypeOfIsSound x₁) :
   GuardedCapabilitiesInvariant (Expr.unaryApp (.is ety) x₁) c₂ request entities ∧
   ∃ v, EvaluatesTo (Expr.unaryApp (.is ety) x₁) request entities v ∧ InstanceOfType v ty
 := by
